proof/correctness/Bytes.ec
@@ -1,0 +1,85 @@
+pragma Goals : printall.
+
+require import AllCore List RealExp IntDiv.
+
+from Jasmin require import JModel.
+
+op W32toBytes (x : W32.t) : W8.t list = rev (to_list (W4u8.unpack8 x)).
+op W32ofBytes (x : W8.t list) : W32.t = W4u8.pack4 (rev x).
+
+import W4u8.
+import W8u8.
+
+lemma W32toBytesK (x : W32.t) :
+    W32ofBytes (W32toBytes x) = x.
+proof.
+rewrite /W32ofBytes /W32toBytes revK /#.
+qed.
+
+op W32toBytes_ext (x : W32.t) (l : int) : W8.t list = 
+  rev (mkseq (fun i => nth W8.zero (to_list (W4u8.unpack8 x)) i) l).
+
+lemma size_W32toBytes (x : W32.t) : 
+    size (W32toBytes x) = 4.
+proof.
+by rewrite /W32toBytes size_rev size_to_list.
+qed.
+
+lemma size_W32toBytes_ext (w : W32.t) (l : int):
+    0 < l => size (W32toBytes_ext w l) = l.
+proof.
+move => ?; rewrite /W32toBytes_ext size_rev size_mkseq /#.
+qed.
+
+lemma W32_toBytes_ext_out (dflt : W8.t) (w : W32.t) (l i : int) :
+    0 < l =>
+    ! (0 <= l - (i + 1) < 4) => 
+    0 <= i < l =>
+    nth dflt (W32toBytes_ext w l) i = W8.zero.
+proof.
+move => ???.
+rewrite /W32toBytes_ext nth_rev; first by rewrite size_mkseq /#.
+rewrite size_mkseq (: max 0 l = l) 1:/#.
+rewrite nth_mkseq 1:/# /=.
+rewrite unpack8E initE ifF //.
+qed.
+
+
+op W64toBytes (x : W64.t) : W8.t list = rev (to_list (W8u8.unpack8 x)).
+op W64ofBytes (x : W8.t list) : W64.t = W8u8.pack8 (rev x).
+
+lemma W64toBytesK (x : W64.t) :
+    W64ofBytes (W64toBytes x) = x.
+proof.
+rewrite /W64ofBytes /W64toBytes revK /#.
+qed.
+
+
+(* Igual ao toByte da spec *)
+op W64toBytes_ext (x : W64.t) (l : int) : W8.t list = 
+  rev (mkseq (fun i => nth W8.zero (to_list (W8u8.unpack8 x)) i) l). 
+
+lemma size_W64toBytes :
+    forall (x : W64.t), size (W64toBytes x) = 8.
+proof.
+by move => ?; rewrite /W64toBytes size_rev size_to_list.
+qed.
+
+
+lemma size_W64toBytes_ext (w : W64.t) (l : int) :
+    0 < l => size (W64toBytes_ext w l) = l.
+proof.
+move => ?; rewrite /W64toBytes_ext size_rev size_mkseq /#.
+qed.
+
+lemma nth_W64toBytes_ext dflt (w : W64.t) (l i : int)  :
+    0 < l => 
+    0 <= i < l =>
+    nth dflt (W64toBytes_ext w l) i = (unpack8 w).[l - (i + 1)]. 
+proof.
+move => ??.
+rewrite /W64toBytes_ext nth_rev; first by rewrite size_mkseq /#.
+rewrite size_mkseq (: max 0 l = l) 1:/# //=.
+by rewrite nth_mkseq 1:/# get_to_list.
+qed.
+
